I. Merging Grammars
- Grammar 1 (L1): Generates strings of the form a<sup>n</sup> (n ≥ 0)
    - S1 → aS1 | ε
- Grammar 2 (L2): Generates strings of the form b<sup>m</sup> (m ≥ 0)
    - S2 → bS2 | ε
- Merged Grammar (L1 ∪ L2):
    - S → S1 | S2
    - S1 → aS1 | ε
    - S2 → bS2 | ε

**Example: Merging for Concatenation**
- Grammar 1 (L1): Generates strings of the form a<sup>n</sup> (n ≥ 0)
    - S1 → aS1 | ε
- Grammar 2 (L2): Generates strings of the form b<sup>m</sup> (m ≥ 0)
    - S2 → bS2 | ε
- Merged Grammar (L1 L2):
    - S → S1 S2
    - S1 → aS1 | ε
    - S2 → bS2 | ε

II. DFA to CFG
• You can convert any DFA into an equivalent CFG as follows. 
	• Make a variable Ri for each state qi of the DFA. 
	• Add the rule Ri → aRj to the CFG if δ(qi,a) = qj is a transition in the DFA. 
	• Add the rule Ri → ε if qi is an accept state of the DFA. 
	• Make R0 the start variable of the grammar, where q0 is the start state of the machine

![[Pasted image 20250317142124.png]]

Example Derivation: 
E ⇒ 0E ⇒ 00E ⇒001O ⇒0010O ⇒00101E ⇒ 001011O ⇒001011