Ambiguity in a grammar refers to a situation where a single string in the language can be derived or parsed in multiple distinct ways. This means that the grammar doesn't provide a unique structural interpretation for the string.

![[Pasted image 20250317142600.png]]

![[Pasted image 20250317142632.png]]


Leftmost Derivation
A derivation of a string w in a grammar G is a leftmost derivation if at every step the leftmost remaining variable is the one replaced. The derivation below is a leftmost derivation.

![[Pasted image 20250317142714.png]]
### Chomsky Normal Form
A CFG is in CNF if all its production rules are in one of the following two forms:
- `A → BC` (where A, B, and C are variables, and B and C are not the start variable)
- `A → a` (where A is a variable, and a is a terminal symbol)
- `S -> ε` (where S is the start variable and ε is the empty string. This is allowed only if the empty string is in the language)

**Converting a CFG to CNF:**
The process of converting a CFG to CNF involves several steps:  
1. **Eliminate ε-productions:**
    - If a variable A can derive ε, remove the rule `A → ε`.
    - For every rule that contains A, add new rules where A is removed.
2. **Eliminate unit productions:**
    - Unit productions are rules of the form `A → B`.
    - Replace each unit production with the production rules of B.
3. **Eliminate useless symbols:**
    - Remove variables and terminals that cannot be derived from the start variable or that do not derive any terminal strings.
4. **Introduce new variables:**
    - For rules of the form `A → a1a2...an` (where n > 1), introduce new variables to replace the terminal symbols.
    - For rules of the form `A → B1B2...Bn` (where n > 2), introduce new variables to break down the rule into binary rules.

**Example:**
Let's say we have the following CFG:
- `S → AB`
- `A → aAA | a`
- `B → bBB | b`

Here's how we might convert it to CNF:
1. **Introduce new variables for terminals:**
    - `S → AB`
    - `A → XAA | a`
    - `B → YBB | b`
    - `X → a`
    - `Y → b`
2. **Introduce new variables for long variable sequences:**
    - `S → AB`
    - `A → XA1 | a`
    - `A1 → AA`
    - `B → YB1 | b`
    - `B1 → BB`
    - `X → a`
    - `Y → b`

This resulting grammar is in CNF.


